

6.4.2.  $\dot{x} = x(3-2x-y) = 0$ ,  $\dot{y} = y(2-x-y) = 0$ , get  $(0,2), (1,1), (\frac{3}{2}, 0), (0,0)$ ,

$$A = \begin{pmatrix} -4x-y+3 & -x \\ -y & -x-2y+2 \end{pmatrix} \quad (0,0) A = \begin{pmatrix} 3 & 0 \\ 0 & 2 \end{pmatrix}$$

$$(0,2) A = \begin{pmatrix} 1 & 0 \\ -2 & -2 \end{pmatrix} \quad \lambda = 1, -2$$

$$(1,1) A = \begin{pmatrix} -2 & -1 \\ -1 & -1 \end{pmatrix} \quad \begin{matrix} \tau = -3 \\ \Delta = 1 \end{matrix} \quad \lambda = \frac{-3 \pm \sqrt{5}}{2}$$

$$(\frac{3}{2}, 0) A = \begin{pmatrix} -3 & -\frac{3}{2} \\ 0 & \frac{1}{2} \end{pmatrix} \quad \begin{matrix} \tau = -\frac{5}{2} \\ \Delta = -\frac{3}{2} \end{matrix} \quad \lambda = -\frac{5}{2} \pm \sqrt{\left(\frac{5}{2}\right)^2 - \frac{3}{2}} \quad \lambda_2 < \lambda_1 < 0$$

